disk-betree/SSTable.dfy
@@ -1,0 +1,397 @@
+include "../lib/sequences.dfy"
+include "../lib/maps.dfy"
+include "../lib/total_order.dfy"
+include "Message.dfy"
+include "PivotBetreeSpec.dfy"
+include "../lib/Marshalling/Native.s.dfy"
+
+module SSTable {
+  import opened ValueMessage
+  import opened Lexicographic_Byte_Order
+  import opened Options
+  import opened Sequences
+  import opened Maps
+  import opened NativeTypes
+  import ValueWithDefault`Internal
+  import Uint64Order = Uint64_Order
+  import BT = PivotBetreeSpec`Internal
+  import P = PivotsLib
+  import Native
+
+  type String = seq<byte>
+  type Key = String
+
+  datatype SSTable = SSTable(starts: seq<uint64>, strings: String)
+
+  function method Start(sst: SSTable, i: uint64) : uint64
+    requires 0 <= i as int < |sst.starts|
+  {
+    sst.starts[i]
+  }
+  
+  function method End(sst: SSTable, i: uint64) : uint64
+    requires |sst.starts| < 0x1000_0000_0000_0000
+    requires 0 <= i as int < |sst.starts|
+    requires |sst.strings| < 0x1_0000_0000_0000_0000
+  {
+    if i + 1 < |sst.starts| as uint64 then
+      sst.starts[i+1]
+    else
+      |sst.strings| as uint64
+  }
+
+  predicate Even(n: int)
+  {
+    n % 2 == 0
+  }
+
+  predicate WFSSTable(sst: SSTable)
+  {
+    && Uint64Order.IsSorted(sst.starts)
+    && |sst.strings| < 0x1000_0000_0000_0000
+    && |sst.starts| < 0x1000_0000_0000_0000
+    && (|sst.starts| > 0 ==> (
+      && sst.starts[0] == 0
+      && 0 <= Last(sst.starts) as int <= |sst.strings|
+    ))
+  }
+
+  lemma LemmaStartEndIndices(sst: SSTable, i: int)
+  requires WFSSTable(sst)
+  requires 0 <= i < |sst.starts|
+  ensures 0 <= Start(sst, i as uint64) as int <= End(sst, i as uint64) as int <= |sst.strings|
+  {
+    Uint64Order.reveal_IsSorted();
+  }
+
+  function method Entry(sst: SSTable, i: int) : String
+  requires WFSSTable(sst)
+  requires 0 <= i as int < |sst.starts|
+  {
+    LemmaStartEndIndices(sst, i);
+
+    sst.strings[Start(sst, i as uint64)..End(sst, i as uint64)]
+  }
+
+  predicate {:opaque} KeysStrictlySorted(sst: SSTable)
+  requires WFSSTable(sst)
+  {
+    forall i, j | 0 <= 2*i < 2*j < |sst.starts| ::
+      lt(Entry(sst, 2*i), Entry(sst, 2*j))
+  }
+
+  predicate WFSSTableMap(sst: SSTable)
+  {
+    && WFSSTable(sst)
+    && Even(|sst.starts|)
+    && KeysStrictlySorted(sst)
+  }
+
+  function {:opaque} IPrefix(sst: SSTable, k: int) : (m : map<String, Message>)
+  requires WFSSTableMap(sst)
+  requires 2*k <= |sst.starts|
+  ensures forall i | 0 <= i < k :: Entry(sst, 2*i) in m && m[Entry(sst, 2*i)] == Define(Entry(sst, 1 + 2*i));
+  ensures forall key | key in m :: exists i :: 0 <= i < k && Entry(sst, 2*i) == key
+
+  function {:opaque} I(sst: SSTable) : (m : map<String, Message>)
+  requires WFSSTableMap(sst)
+  ensures forall i | 0 <= 2*i < |sst.starts| :: Entry(sst, 2*i) in m && m[Entry(sst, 2*i)] == Define(Entry(sst, 1 + 2*i));
+  ensures forall key | key in m :: exists i :: 0 <= 2*i < |sst.starts| && Entry(sst, 2*i) == key
+
+  function ISeq(ssts: seq<SSTable>) : (res : seq<map<String, Message>>)
+  requires forall i | 0 <= i < |ssts| :: WFSSTableMap(ssts[i])
+  ensures |res| == |ssts|
+  ensures forall i | 0 <= i < |ssts| :: I(ssts[i]) == res[i]
+
+  method Cmp(key: Key, sst: SSTable, i: uint64) returns (c: int32)
+  requires WFSSTable(sst)
+  requires 0 <= i as int < |sst.starts|
+  ensures c == 0 || c == -1 || c == 1
+  ensures c == 0 ==> key == Entry(sst, i as int)
+  ensures c == -1 ==> lt(key, Entry(sst, i as int))
+  ensures c == 1 ==> lt(Entry(sst, i as int), key)
+  {
+    reveal_seq_lte();
+    Base_Order.reveal_lte();
+
+    var j: uint64 := 0;
+    var start: uint64 := Start(sst, i);
+    var end: uint64 := End(sst, i);
+
+    LemmaStartEndIndices(sst, i as int);
+    assert |Entry(sst, i as int)| == end as int - start as int;
+
+    while j as int < |key| && start + j < end
+    invariant 0 <= j
+    invariant j as int <= |key|
+    invariant start as int + j as int <= end as int
+    invariant seq_lte(key[j..], Entry(sst, i as int)[j..]) ==> seq_lte(key, Entry(sst, i as int))
+    invariant seq_lte(Entry(sst, i as int)[j..], key[j..]) ==> seq_lte(Entry(sst, i as int), key)
+    invariant key[..j] == Entry(sst, i as int)[..j];
+    {
+      if key[j] < sst.strings[start + j] {
+        //assert key[j] == key[j..][0];
+        //assert sst.strings[start + j] == Entry(sst, i)[j..][0];
+        //assert key[j..][0] < Entry(sst, i)[j..][0];
+        //assert Base_Order.lt(key[j..][0], Entry(sst, i)[j..][0]);
+        //assert seq_lte(key[j..], Entry(sst, i)[j..]);
+        return -1;
+      }
+      if key[j] > sst.strings[start + j] {
+        return 1;
+      }
+      j := j + 1;
+    }
+
+    if start + j < end {
+      assert j as int == |key|;
+      return -1;
+    }
+    if j as int < |key| {
+      assert start + j == end;
+      return 1;
+    }
+
+    assert j as int == |key|;
+    assert start + j == end;
+    return 0;
+  }
+
+  method Cmp2(sst: SSTable, i: uint64, sst': SSTable, j: uint64) returns (c: int32)
+  requires WFSSTable(sst)
+  requires WFSSTable(sst')
+  requires 0 <= i as int < |sst.starts|
+  requires 0 <= j as int < |sst'.starts|
+  ensures c == 0 || c == -1 || c == 1
+  ensures c == 0 ==> Entry(sst, i as int) == Entry(sst', j as int)
+  ensures c == -1 ==> lt(Entry(sst, i as int), Entry(sst', j as int))
+  ensures c == 1 ==> lt(Entry(sst', j as int), Entry(sst, i as int))
+
+
+  lemma IndicesLtOfKeysLt(sst: SSTable, i: int, j: int)
+  requires WFSSTableMap(sst)
+  requires 0 <= 2*i < |sst.starts|
+  requires 0 <= 2*j < |sst.starts|
+  requires lt(Entry(sst, 2*i), Entry(sst, 2*j))
+  ensures i < j
+  {
+    reveal_KeysStrictlySorted();
+  }
+
+  method Query(sst: SSTable, key: Key) returns (m: Option<Message>)
+  requires WFSSTableMap(sst)
+  ensures m.None? ==> key !in I(sst)
+  ensures m.Some? ==> key in I(sst) && I(sst)[key] == m.value
+  {
+    var lo: uint64 := 0;
+    var hi: uint64 := (|sst.starts| as uint64) / 2;
+
+    while lo < hi
+    invariant 0 <= 2*lo as int <= |sst.starts|
+    invariant 0 <= 2*hi as int <= |sst.starts|
+    invariant lo > 0 ==> lt(Entry(sst, 2*(lo-1) as int), key)
+    invariant 2*hi as int < |sst.starts| ==> lt(key, Entry(sst, 2*hi as int))
+    decreases hi as int - lo as int
+    {
+      var mid: uint64 := (lo + hi) / 2;
+      var c := Cmp(key, sst, 2*mid);
+      if c == 0 {
+        m := Some(Define(Entry(sst, 2*mid as int + 1)));
+        return;
+      } else if (c == -1) {
+        hi := mid;
+      } else {
+        lo := mid + 1;
+      }
+    }
+
+    if (key in I(sst)) {
+      ghost var j :| 0 <= 2*j < |sst.starts| && Entry(sst, 2*j as int) == key;
+      if (lo > 0) { IndicesLtOfKeysLt(sst, lo as int - 1, j as int); }
+      if (2*hi as int < |sst.starts|) { IndicesLtOfKeysLt(sst, j as int, hi as int); }
+    }
+
+    m := None;
+  }
+
+  /*
+  method Merge(l: SSTable, r: SSTable) returns (c: SSTable)
+  requires WFSSTableMap(l)
+  requires WFSSTableMap(r)
+  requires forall keyl, keyr | keyl in I(l) && keyr in I(r) :: lt(keyl, keyr)
+  ensures I(c) == MapDisjointUnion(I(l), I(r))
+  */
+
+  predicate WFSSTableMapArrays(starts: array<uint64>, startsIdx: uint64, strings: array<byte>, stringsIdx: uint64)
+  reads starts
+  reads strings
+  requires 0 <= startsIdx as int <= starts.Length
+  requires 0 <= stringsIdx as int <= strings.Length
+  {
+    WFSSTableMap(SSTable(starts[..startsIdx], strings[..stringsIdx]))
+  }
+
+  function IArrays(starts: array<uint64>, startsIdx: uint64, strings: array<byte>, stringsIdx: uint64) : map<Key, Message>
+  reads starts
+  reads strings
+  requires 0 <= startsIdx as int <= starts.Length
+  requires 0 <= stringsIdx as int <= strings.Length
+  requires WFSSTableMapArrays(starts, startsIdx, strings, stringsIdx)
+  {
+    I(SSTable(starts[..startsIdx], strings[..stringsIdx]))
+  }
+
+  method MaxLens(s: seq<SSTable>)
+  returns (startsLen : uint64, stringsLen: uint64)
+  ensures forall i | 0 <= i < |s| :: |s[i].starts| <= startsLen as int
+  ensures forall i | 0 <= i < |s| :: |s[i].strings| <= stringsLen as int
+
+  lemma LemmaStartsArrayIsStrictlySorted(startsArray: array<uint64>, startsIdx: int, stringsIdx: int)
+  requires 0 <= startsIdx
+  requires startsIdx + 2 <= startsArray.Length
+  requires Uint64Order.IsSorted(startsArray[..startsIdx])
+  requires startsArray[startsIdx] as int == stringsIdx
+  requires startsArray[startsIdx + 1] as int >= stringsIdx
+  requires forall j | 0 <= j < startsIdx :: startsArray[j] as int <= stringsIdx
+  ensures Uint64Order.IsSorted(startsArray[..startsIdx + 2])
+  {
+    Uint64Order.reveal_IsSorted();
+  }
+
+  method LemmaAugmentSSTable(sst: SSTable, sst': SSTable)
+  requires WFSSTableMap(sst)
+  requires WFSSTableMap(sst')
+  requires |sst'.starts| == |sst.starts| + 2
+  requires sst.starts == sst'.starts[..|sst.starts|]
+  requires sst.strings == sst'.strings[..|sst.strings|]
+  ensures I(sst) == I(sst')
+  {
+  }
+
+  method WriteKeyValue(startsArray: array<uint64>, stringsArray: array<byte>, startsIdx: uint64, stringsIdx: uint64, sst: SSTable, i: uint64)
+  returns (startsIdx': uint64, stringsIdx': uint64)
+  modifies startsArray
+  modifies stringsArray
+  requires WFSSTableMap(sst)
+  requires 0 <= i
+  requires i as int + 1 < |sst.starts|
+  requires 0 <= startsIdx
+  requires startsIdx as int + 2 <= startsArray.Length
+  requires 0 <= stringsIdx
+  requires stringsIdx as int <= stringsArray.Length
+  requires stringsIdx as int + End(sst, i+1) as int - Start(sst, i) as int <= stringsArray.Length
+  requires WFSSTableMapArrays(startsArray, startsIdx, stringsArray, stringsIdx)
+  requires forall key | key in IArrays(startsArray, startsIdx, stringsArray, stringsIdx) :: lt(key, Entry(sst, i as int))
+  requires forall j | 0 <= j < startsIdx :: startsArray[j] <= stringsIdx
+  requires stringsArray.Length < 0x1000_0000_0000_0000
+  requires startsArray.Length < 0x1000_0000_0000_0000
+  requires startsIdx == 0 ==> stringsIdx == 0
+  ensures 0 <= startsIdx' as int <= startsArray.Length
+  ensures 0 <= stringsIdx' as int <= stringsArray.Length
+  ensures WFSSTableMapArrays(startsArray, startsIdx', stringsArray, stringsIdx')
+  ensures IArrays(startsArray, startsIdx', stringsArray, stringsIdx')
+       == old(IArrays(startsArray, startsIdx, stringsArray, stringsIdx))[Entry(sst, i as int) := Define(Entry(sst, i as int + 1))]
+  {
+    LemmaStartEndIndices(sst, i as int);
+    LemmaStartEndIndices(sst, i as int + 1);
+
+    startsArray[startsIdx] := stringsIdx;
+    startsArray[startsIdx + 1] := stringsIdx + (End(sst, i) - Start(sst, i));
+    startsIdx' := startsIdx + 2;
+
+    Native.Arrays.CopySeqIntoArray(sst.strings, Start(sst, i), stringsArray, stringsIdx, End(sst, i+1) - Start(sst, i));
+    stringsIdx' := stringsIdx + End(sst, i+1) - Start(sst, i);
+
+    LemmaStartsArrayIsStrictlySorted(startsArray, startsIdx as int, stringsIdx as int);
+
+    assert startsArray[..startsIdx] == old(startsArray[..startsIdx]);
+    assert stringsArray[..stringsIdx] == old(stringsArray[..stringsIdx]);
+    assert old(IArrays(startsArray, startsIdx, stringsArray, stringsIdx))
+        == IArrays(startsArray, startsIdx, stringsArray, stringsIdx);
+    assert WFSSTableMapArrays(startsArray, startsIdx, stringsArray, stringsIdx);
+    
+  }
+
+  method Flush(parent: SSTable, children: seq<SSTable>, pivots: seq<Key>)
+  returns (res : seq<SSTable>)
+  requires |children| == |pivots| + 1
+  requires forall i, key | 0 <= i < |children| && key in I(children[i]) :: P.Route(pivots, key) == i
+  //ensures |res| == |children|
+  //ensures forall i, key | 0 <= i < |res| && key in I(res[i]) ==> Route(pivots, key) == i
+  ensures ISeq(res) == BT.AddMessagesToBuckets(pivots, |children|, ISeq(children), I(parent))
+  {
+    var maxChildStartsLen: uint64, maxChildStringsLen: uint64 := MaxLens(children);
+    var startsArray : array<uint64> := new uint64[maxChildStartsLen + |parent.starts| as uint64];
+    var stringsArray : array<byte> := new byte[maxChildStringsLen + |parent.strings| as uint64];
+    var startsIdx: uint64 := 0;
+    var stringsIdx: uint64 := 0;
+
+    res := [];
+
+    var parentIdx: uint64 := 0;
+    var childrenIdx: int := 0;
+    var childIdx: uint64 := 0;
+    while childrenIdx < |children|
+    invariant 0 <= 2*parentIdx as int <= |parent.starts|
+    invariant 0 <= childrenIdx <= |children|
+    invariant childrenIdx < |children| ==> 0 <= 2*childIdx as int <= |children[childrenIdx].starts|
+    invariant 0 <= startsIdx as int <= startsArray.Length
+    invariant 0 <= stringsIdx as int <= stringsArray.Length
+    invariant 2*parentIdx as int < |parent.starts| ==>
+        forall key | key in IArrays(startsArray, startsIdx, stringsArray, stringsIdx) :: lt(key, Entry(parent, 2*parentIdx as int))
+    invariant childrenIdx < |children| && 2*childIdx as int < |children[childrenIdx].starts| ==>
+        forall key | key in IArrays(startsArray, startsIdx, stringsArray, stringsIdx) :: lt(key, Entry(children[childrenIdx], 2*childIdx as int))
+    invariant WFSSTableMapArrays(startsArray, startsIdx, stringsArray, stringsIdx)
+    invariant IArrays(startsArray, startsIdx, stringsArray, stringsIdx)
+           == BT.AddMessagesToBucket(pivots, childrenIdx, IPrefix(children[childrenIdx], childIdx as int), IPrefix(parent, parentIdx as int))
+    invariant ISeq(res) == BT.AddMessagesToBuckets(pivots, |res|, ISeq(children), I(parent))
+    {
+      if (2*parentIdx == |parent.starts| as uint64) {
+        if (2*childIdx == |children[childrenIdx].starts| as uint64) {
+          res := res + [SSTable(startsArray[..startsIdx], stringsArray[..stringsIdx])];
+
+          startsIdx := 0;
+          stringsIdx := 0;
+          childIdx := 0;
+          childrenIdx := childrenIdx + 1;
+        } else {
+          startsIdx, stringsIdx := WriteKeyValue(startsArray, stringsArray, startsIdx, stringsIdx, children[childrenIdx], 2*childIdx);
+          childIdx := childIdx + 1; 
+        }
+      } else {
+        if (2*childIdx == |children[childrenIdx].starts| as uint64) {
+          if (childrenIdx == |children| - 1) {
+            startsIdx, stringsIdx := WriteKeyValue(startsArray, stringsArray, startsIdx, stringsIdx, parent, 2*parentIdx);
+            parentIdx := parentIdx + 1;
+          } else {
+            var c := Cmp(pivots[childrenIdx], parent, 2*parentIdx);
+            if (c == -1) {
+              startsIdx, stringsIdx := WriteKeyValue(startsArray, stringsArray, startsIdx, stringsIdx, parent, 2*parentIdx);
+              parentIdx := parentIdx + 1;
+            } else {
+              res := res + [SSTable(startsArray[..startsIdx], stringsArray[..stringsIdx])];
+
+              startsIdx := 0;
+              stringsIdx := 0;
+              childIdx := 0;
+              childrenIdx := childrenIdx + 1;
+            }
+          }
+        } else {
+          var c := Cmp2(parent, 2*parentIdx as uint64, children[childrenIdx], 2*childIdx as uint64);
+          if (c == 0) {
+            startsIdx, stringsIdx := WriteKeyValue(startsArray, stringsArray, startsIdx, stringsIdx, parent, 2*parentIdx);
+            childIdx := childIdx + 1;
+            parentIdx := parentIdx + 1;
+          } else if (c == -1) {
+            startsIdx, stringsIdx := WriteKeyValue(startsArray, stringsArray, startsIdx, stringsIdx, parent, 2*parentIdx);
+            parentIdx := parentIdx + 1;
+          } else if (c == 1) {
+            startsIdx, stringsIdx := WriteKeyValue(startsArray, stringsArray, startsIdx, stringsIdx, children[childrenIdx], 2*childIdx);
+            childIdx := childIdx + 1; 
+          }
+        }
+      }
+    }
+  }
+}
